Proofs/Memory_Nodes.thy
@@ -1,0 +1,64 @@
+theory Memory_Nodes
+  imports
+    "../AutoCorres/Impl"
+    "../lib/ExtraLemmas"
+begin
+  
+context sable_isa
+begin
+  
+abbreviation node_size
+  where "node_size s n \<equiv> size_C (h_val (hrs_mem (t_hrs_' s)) n)"
+abbreviation node_size_masked
+  where "node_size_masked s n \<equiv> (node_size s n) && scast (~~ MEM_NODE_OCCUPIED_FLAG)"
+    
+abbreviation node_next
+  where "node_next s n \<equiv> next_C (h_val (hrs_mem (t_hrs_' s)) n)" 
+abbreviation node_is_occupied
+  where "node_is_occupied s n \<equiv> (mem_node_C.size_C (h_val (hrs_mem (t_hrs_' s)) n)) && scast  MEM_NODE_OCCUPIED_FLAG"
+    
+abbreviation update_node :: " globals \<Rightarrow> mem_node_C ptr \<Rightarrow> mem_node_C \<Rightarrow> globals"
+  where "update_node s n node_val \<equiv>
+  (t_hrs_'_update (hrs_mem_update (heap_update n node_val)) s)"
+value t_hrs_'_update
+  
+abbreviation hrs_the_same_at
+  where "hrs_the_same_at s s' p \<equiv>
+  fst (t_hrs_' s) p = fst (t_hrs_' s') p \<and> snd (t_hrs_' s) p = snd (t_hrs_' s') p"
+lemma t_hrs_'_t_hrs_'_update_simp:
+  "t_hrs_' (t_hrs_'_update m (s::globals)) = m (t_hrs_' s)" by simp
+    
+lemma updated_node_val: 
+  "h_val (hrs_mem (t_hrs_' (update_node s n node_val))) n = node_val"
+  by (simp add: h_val_heap_update hrs_mem_update)
+    
+lemma updated_node_size:
+  "node_size (update_node s n (mem_node_C nodeSize next)) n = nodeSize"
+  using sable_isa.updated_node_val by auto
+    
+lemma updated_node_next:
+  "node_next (update_node s n (mem_node_C nodeSize next)) n = next"
+  using sable_isa.updated_node_val by auto
+    
+lemma hrs_the_same_nodes_the_same:
+  "\<forall>p \<in> {ptr_val (node::mem_node_C ptr)..+size_of (TYPE(mem_node_C))}. hrs_the_same_at s s' p \<Longrightarrow>
+    (h_val (hrs_mem (t_hrs_' s)) node) = (h_val (hrs_mem (t_hrs_' s')) node)"
+  unfolding h_val_def hrs_mem_def
+  apply (subgoal_tac " heap_list (fst (t_hrs_' s)) (size_of TYPE(mem_node_C)) (ptr_val node) =
+     heap_list (fst (t_hrs_' s')) (size_of TYPE(mem_node_C)) (ptr_val node)")
+   apply auto
+  apply (rule heap_list_h_eq2)
+  by simp
+    
+lemma MEM_NODE_OCCUPIED_FLAG_not_zero:
+  "MEM_NODE_OCCUPIED_FLAG \<noteq> (0:: 32 signed word)" unfolding MEM_NODE_OCCUPIED_FLAG_def by auto
+
+lemma one_mask_neg_MNOF_not_zero[simp]:
+  "(1::32 signed word) && ~~ MEM_NODE_OCCUPIED_FLAG = (0::32 signed word) \<Longrightarrow> False"
+     unfolding MEM_NODE_OCCUPIED_FLAG_def by unat_arith
+
+end
+  
+end
+  
+  
